veric/mpred.v
@@ -413,7 +413,7 @@ Class funspecGS Σ := FunspecG {
 
 Class heapGS Σ := HeapGS {
   heapGS_invGS :> invGS_gen HasNoLc Σ;
-  heapGS_gen_heapGS :> gen_heapGS address resource Σ;
+  heapGS_gen_heapGS :> gen_heapGS share address resource Σ;
   heapGS_funspecGS :> funspecGS Σ
 }.
 
@@ -534,7 +534,7 @@ Ltac super_unfold_lift :=
   cbv delta [liftx LiftEnviron LiftAEnviron Tarrow Tend lift_S lift_T lift_prod
   lift_last lifted lift_uncurry_open lift_curry lift lift0 lift1 lift2 lift3 alift0 alift1 alift2 alift3] beta iota in *.
 
-(* switch from an entailment on asserts to mpreds *)
+(* switch from an entailment on asserts to mpreds; mostly the same as monPred.unseal *)
 Ltac raise_rho :=
   try (constructor; intro rho); 
   repeat (rewrite monPred_at_and ||
